zoo_saturn/mpmc_queue_2: Remove [push_front] and fix invariant.

lib/zoo_saturn/mpmc_queue_2.ml
@@ -2,43 +2,43 @@
    https://github.com/ocaml-multicore/picos/blob/0c8d97df54b319ed4a7857d66f801b18a9e76f38/lib/picos_aux.mpmcq/picos_aux_mpmcq.ml
 *)
 
-type ('a, _) front =
+type ('a, _) suffix =
   | Front :
     int ->
-    ('a, [> `Front]) front
+    ('a, [> `Front]) suffix
   | Cons :
-    int * 'a * ('a, [`Front | `Cons]) front ->
-    ('a, [> `Cons]) front
+    int * 'a * ('a, [`Front | `Cons]) suffix ->
+    ('a, [> `Cons]) suffix
     [@generative]
 
-type ('a, _) back =
+type ('a, _) prefix =
   | Back :
     { index: int;
-      mutable move: ('a, [`Snoc | `Used]) back;
+      mutable move: ('a, [`Snoc | `Used]) prefix;
     } ->
-    ('a, [> `Back]) back
+    ('a, [> `Back]) prefix
   | Snoc :
-    int * 'a * ('a, [`Back | `Snoc]) back ->
-    ('a, [> `Snoc]) back
+    int * 'a * ('a, [`Back | `Snoc]) prefix ->
+    ('a, [> `Snoc]) prefix
     [@generative]
   | Used :
-    ('a, [> `Used]) back
+    ('a, [> `Used]) prefix
 
 type 'a t =
-  { mutable front: ('a, [`Front | `Cons]) front [@atomic];
-    mutable back: ('a, [`Back | `Snoc]) back [@atomic];
+  { mutable front: ('a, [`Front | `Cons]) suffix [@atomic];
+    mutable back: ('a, [`Back | `Snoc]) prefix [@atomic];
   }
 
-let rec rev (suffix : (_, [< `Cons]) front) prefix =
-  let Cons _ as suffix = suffix in
-  match prefix with
+let rec rev (suff : (_, [< `Cons]) suffix) pref =
+  let Cons _ as suff = suff in
+  match pref with
   | Back _ ->
-      suffix
-  | Snoc (i, v, prefix) ->
-      rev (Cons (i, v, suffix)) prefix
-let rev (back : (_, [< `Snoc]) back) =
-  let Snoc (i, v, prefix) = back in
-  rev (Cons (i, v, Front (i + 1))) prefix
+      suff
+  | Snoc (i, v, pref) ->
+      rev (Cons (i, v, suff)) pref
+let rev (back : (_, [< `Snoc]) prefix) =
+  let Snoc (i, v, pref) = back in
+  rev (Cons (i, v, Front (i + 1))) pref
 
 let create () =
   { front= Front 1;
@@ -71,7 +71,7 @@ let rec size t =
 let is_empty t =
   size t == 0
 
-let finish (back : (_, [< `Back]) back) =
+let finish (back : (_, [< `Back]) prefix) =
   let Back back_r = back in
   back_r.move <- Used
 
@@ -85,63 +85,23 @@ let help t back i_move move =
   | _ ->
       finish back
 
-let rec push_back_aux t v i back =
+let rec push_aux t v i back =
   let new_back = Snoc (i + 1, v, back) in
   if not @@ Atomic.Loc.compare_and_set [%atomic.loc t.back] back new_back then (
     Domain.yield () ;
-    push_back t v
+    push t v
   )
-and push_back t v =
+and push t v =
   match t.back with
   | Snoc (i, _, _) as back ->
-      push_back_aux t v i back
+      push_aux t v i back
   | Back back_r as back ->
       match back_r.move with
       | Used ->
-          push_back_aux t v back_r.index back
+          push_aux t v back_r.index back
       | Snoc (i_move, _, _) as move ->
           help t back i_move move ;
-          push_back t v
-
-let rec push_front t v =
-  match t.front with
-  | Cons (i, _, _) as front ->
-      let new_front = Cons (i - 1, v, front) in
-      if not @@ Atomic.Loc.compare_and_set [%atomic.loc t.front] front new_front then (
-        Domain.yield () ;
-        push_front t v
-      )
-  | Front i_front as front ->
-      match t.back with
-      | Snoc (i_back, v_back, prefix) as back ->
-          if t.front != front then (
-            push_front t v
-          ) else if i_front == i_back then (
-            let new_back = Snoc (i_back + 1, v_back, Snoc (i_back, v, prefix)) in
-            if not @@ Atomic.Loc.compare_and_set [%atomic.loc t.back] back new_back then (
-              Domain.yield () ;
-              push_front t v
-            )
-          ) else (
-            let new_back = Back { index= i_back; move= back } in
-            if not @@ Atomic.Loc.compare_and_set [%atomic.loc t.back] back new_back then
-              Domain.yield () ;
-            push_front t v
-          )
-      | Back back_r as back ->
-          match back_r.move with
-          | Used ->
-              if t.front != front then
-                push_front t v
-              else
-                let new_back = Snoc (back_r.index + 1, v, back) in
-                if not @@ Atomic.Loc.compare_and_set [%atomic.loc t.back] back new_back then (
-                  Domain.yield () ;
-                  push_front t v
-                )
-          | Snoc (i_move, _, _) as move ->
-              help t back i_move move ;
-              push_front t v
+          push t v
 
 let rec pop_1 t front =
   match front with
@@ -154,14 +114,14 @@ let rec pop_1 t front =
       )
   | Front i_front as front ->
       match t.back with
-      | Snoc (i_move, v, move_prefix) as move ->
+      | Snoc (i_move, v, move_pref) as move ->
           if i_front == i_move then (
-            if Atomic.Loc.compare_and_set [%atomic.loc t.back] move move_prefix then
+            if Atomic.Loc.compare_and_set [%atomic.loc t.back] move move_pref then
               Some v
             else
               pop t
           ) else (
-            let (Back _ as back : (_, [`Back]) back) = Back { index= i_move; move } in
+            let (Back _ as back : (_, [`Back]) prefix) = Back { index= i_move; move } in
             let front' = t.front in
             if front' != front then
               pop_1 t front'
@@ -181,7 +141,7 @@ let rec pop_1 t front =
               else
                 pop_3 t proph front
 and pop_2 t front back move =
-  let (Cons (_, v, new_front) : (_, [`Cons]) front) = rev move in
+  let (Cons (_, v, new_front) : (_, [`Cons]) suffix) = rev move in
   if Atomic.Loc.compare_and_set [%atomic.loc t.front] front new_front then (
     finish back ;
     Some v
